ImpLang parsing without running

LeanGoa/QuickSort.lean
@@ -16,43 +16,64 @@ Our implementation of quicksort for lists follows the following steps:
 We begin by defining `smaller` and `larger` lists. We define them as abbreviations so that they are automatically unfolded by Lean.
 -/
 
-
-/-!
-We define `smaller` and `larger` using `List.filter`. We need some theorems relating to filtering.
--/
 variable {α : Type}[LinearOrder α]
 
-@[simp, grind]
+@[grind]
 def smaller (pivot : α) (l : List α) : List α :=
   l.filter (fun x => x ≤  pivot)
 
-@[simp, grind]
+@[grind]
 def larger (pivot : α) (l : List α) : List α :=
   l.filter (fun x => pivot < x)
 
 def quickSort : List α → List α
-  | _ => sorry
+  | [] => []
+  | pivot :: l =>
+    have hs : (smaller pivot l).length < (pivot :: l).length := by
+      grind
+    have hl : (larger pivot l).length < (pivot :: l).length := by
+      grind
+    (quickSort (smaller pivot l)) ++ pivot :: (quickSort (larger pivot l))
+termination_by l => l.length
 
 
 @[simp, grind]
 theorem quickSort_nil : quickSort ([] : List α) = [] := by
-  sorry
+  simp [quickSort]
 
 @[simp, grind]
 theorem quickSort_cons (pivot : α) (l : List α) :
     quickSort (pivot :: l) = (quickSort (smaller pivot l)) ++
     pivot :: (quickSort (larger pivot l)) := by
-  sorry
+  simp [quickSort]
 
 @[grind]
 theorem mem_iff_below_or_above_pivot (pivot : α)
   (l : List α)(x : α) :
     x ∈ l ↔ x ∈ smaller pivot l ∨ x ∈ larger pivot l := by
-  sorry
+  apply Iff.intro
+  · intro h
+    if h' : x ≤ pivot then
+      grind
+    else
+      simp only [not_le] at h'
+      grind
+  · grind
 
 theorem mem_iff_mem_quickSort (l: List α)(x : α) :
     x ∈ l ↔ x ∈ quickSort l := by
-  sorry
+  cases l with
+  | nil =>
+    simp
+  | cons pivot l =>
+    have : (smaller pivot l).length < (pivot :: l).length := by
+      grind
+    have : (larger pivot l).length < (pivot :: l).length := by
+      grind
+    have ihb := mem_iff_mem_quickSort (smaller pivot l)
+    have iha := mem_iff_mem_quickSort (larger pivot l)
+    grind
+termination_by l.length
 
 inductive Sorted : List α → Prop
   | nil : Sorted []
@@ -63,11 +84,30 @@ inductive Sorted : List α → Prop
 @[grind]
 theorem head_le_of_sorted  (a: α) (l : List α) :
   Sorted (a :: l) → ∀ x ∈ l, a ≤ x := by
-  sorry
+  intro h
+  match h with
+  | Sorted.singleton .. => simp
+  | Sorted.step .(a) y l hxy tail_sorted =>
+    intro z hz
+    simp at hz
+    cases hz
+    · grind
+    · have ih := head_le_of_sorted y l tail_sorted
+      trans y
+      · assumption
+      · grind
 
+@[grind]
 theorem cons_sorted (l : List α) :  Sorted l → (a : α) →
   (∀ y ∈ l, a ≤ y) → Sorted (a :: l)  := by
-  sorry
+  intro h₁ a h₀
+  match l with
+  | [] =>
+    apply Sorted.singleton
+  | x :: l' =>
+    apply Sorted.step a x
+    · grind
+    · assumption
 
 theorem sorted_sandwitch (l₁ : List α) (h₁ : Sorted l₁)
     (l₂ : List α) (h₂ : Sorted l₂)
@@ -75,30 +115,35 @@ theorem sorted_sandwitch (l₁ : List α) (h₁ : Sorted l₁)
     (h_bound₁ : ∀ x ∈ l₁, x ≤ bound)
     (h_bound₂ : ∀ x ∈ l₂, bound ≤ x) :
     Sorted (l₁ ++ bound :: l₂) := by
-  sorry
+    induction h₁ with
+    | nil => grind
+    | singleton x =>
+      simp only [List.cons_append, List.nil_append]
+      apply Sorted.step <;> grind
+    | step x y l hxy tail_sorted ih =>
+      simp only [List.cons_append]
+      apply Sorted.step <;> grind
 
 theorem quickSort_sorted (l : List α) : Sorted (quickSort l) := by
-  sorry
--- Exploration commands
+  cases l with
+  | nil =>
+    simp [quickSort_nil]
+    apply Sorted.nil
+  | cons pivot l =>
+    rw [quickSort_cons]
+    apply sorted_sandwitch
+    · have : (smaller pivot l).length < (pivot :: l).length :=
+        by grind
+      apply quickSort_sorted (smaller pivot l)
+    · have : (larger pivot l).length < (pivot :: l).length :=
+        by grind
+      apply quickSort_sorted (larger pivot l)
+    · intro x
+      rw [← mem_iff_mem_quickSort]
+      grind
+    · intro x
+      rw [← mem_iff_mem_quickSort]
+      grind [le_of_lt]
+termination_by l.length
 
-set_option pp.match false in
-set_option pp.proofs false in
-set_option pp.fieldNotation false in
-#print quickSort
-
-set_option pp.match false in
-set_option pp.proofs false in
-#print quickSort.match_1
-
-#print WellFounded
-#check invImage
-/-
-{α : Sort u} →
-  {C : α → Sort v} → {r : α → α → Prop} → WellFounded r → ((x : α) → ((y : α) → r y x → C y) → C x) → (x : α) → C x
--/
-#check WellFounded.fix
-
-/- {α : Sort u} →
-  {r : α → α → Prop} → WellFounded r → {C : α → Sort v} → (a : α) → ((x : α) → ((y : α) → r y x → C y) → C x) → C a
--/
-#check WellFounded.recursion
+#eval quickSort [3,6,8,10,1,2,1]
