LeanGoa/ImpLang.lean
@@ -1,0 +1,150 @@
+import Lean
+import Std
+
+open Lean Meta Elab Term
+
+/-!
+# IMP: A tiny imperative language
+
+* Int ::= the domain of (unbounded) integer numbers, with usual operations on them
+* Bool ::= the domain of Booleans Id ::= standard identifiers
+* AExp ::= Int | Id |  AExp + AExp | AExp / AExp * BExp ::= Bool | AExp <= AExp | | !BExp | BExp && BExp
+
+* Block ::= {} | { Stmt}
+* Stmt ::= Block | Id = AExp; | Stmt Stmt | if(BExp) Block else Block | while(BExp) Block
+* Pgm ::= int List{Id}; Stmt
+
+- When we run a program, we only change state
+- We can drop the requirement of declaration in advance, so we just have statements.
+-/
+namespace ImpLang
+
+-- variables with name
+abbrev ImpLangM :=
+  StateT  (Std.HashMap Name Int) TermElabM
+
+def getVar (name: Name) : ImpLangM Int := do
+  let m ← get
+  return m.get! name
+
+def setVar (name : Name) (value : Int) :
+  ImpLangM Unit := do
+  modify (fun m => m.insert name value)
+
+declare_syntax_cat arith_exp
+syntax num : arith_exp
+syntax ident : arith_exp
+syntax arith_exp "+" arith_exp : arith_exp
+syntax arith_exp "/" arith_exp : arith_exp
+syntax "(" arith_exp ")" : arith_exp
+
+declare_syntax_cat bool_exp
+syntax "T" : bool_exp
+syntax "F" : bool_exp
+syntax "!" bool_exp:70 : bool_exp
+syntax bool_exp:35 "&&" bool_exp:36 : bool_exp
+syntax "(" bool_exp ")" : bool_exp
+syntax arith_exp "≤" arith_exp : bool_exp
+
+declare_syntax_cat imp_statement
+
+syntax imp_block := "{" (imp_statement)? "}"
+
+syntax imp_block : imp_statement
+
+syntax imp_statement imp_statement : imp_statement
+
+syntax ident ":=" arith_exp ";" : imp_statement
+
+syntax "if" ppSpace "(" bool_exp ")" ppSpace imp_block "else" imp_block : imp_statement
+
+syntax "while" "(" bool_exp ")" ppSpace imp_block : imp_statement
+
+inductive Statement where
+| block (s: Option Statement)
+| pair (first second: Statement)
+| assignment (var: Name) (value: Int)
+| if_statement (condition: Bool)
+  (then_statement else_statement : Option Statement)
+| while_statement (condition: Bool) (body: Option Statement)
+deriving Repr, Inhabited, ToExpr
+
+partial def getIntM : TSyntax `arith_exp → ImpLangM Int
+| `(arith_exp| ($e)) => getIntM e
+| `(arith_exp| $n:num) => return n.getNat
+| `(arith_exp| $a:arith_exp + $b:arith_exp) => do
+  let aInt ← getIntM a
+  let bInt ← getIntM b
+  return aInt + bInt
+| `(arith_exp| $a:arith_exp / $b:arith_exp) => do
+  let aInt ← getIntM a
+  let bInt ← getIntM b
+  return aInt / bInt
+| `(arith_exp| $n:ident) => do
+  getVar n.getId
+| _ => Elab.throwUnsupportedSyntax
+
+partial def getBoolM : TSyntax `bool_exp → ImpLangM Bool
+| `(bool_exp| T) => return true
+| `(bool_exp| F) => return false
+| `(bool_exp| ! $b) => do
+  let bVal ← getBoolM b
+  return ¬bVal
+| `(bool_exp| $b && $b' ) => do
+  let bVal ← getBoolM b
+  let bVal' ← getBoolM b'
+  return bVal && bVal'
+| `(bool_exp | $x:arith_exp ≤ $y:arith_exp) => do
+  let xVal ← getIntM x
+  let yVal ← getIntM y
+  return xVal ≤ yVal
+| `(bool_exp| ($b)) => getBoolM b
+| _ => throwUnsupportedSyntax
+
+partial def getStatementM :
+  TSyntax `imp_statement → ImpLangM Statement
+| `(imp_statement| {}) => return .block (none)
+| `(imp_statement| {$s}) => do
+  let stat ← getStatementM s
+  return .block (some stat)
+| `(imp_statement| $s₁ $s₂) => do
+  let stat₁ ← getStatementM s₁
+  let stat₂ ← getStatementM s₂
+  return .pair stat₁ stat₂
+| `(imp_statement| $name:ident := $val ;) => do
+  let value ← getIntM val
+  return .assignment name.getId value
+| `(imp_statement| if ($p) $t else $e) => do
+  let c ← getBoolM p
+  let then_block ← getBlockM t
+  let else_block ← getBlockM e
+  return .if_statement c then_block else_block
+| `(imp_statement| while ($p) $b) => do
+  let c ← getBoolM p
+  let body ← getBlockM b
+  return .while_statement c body
+| _ => throwUnsupportedSyntax
+where getBlockM (bs : TSyntax ``imp_block): ImpLangM (Option Statement) :=
+  match bs with
+  | `(imp_block| {}) => return none
+  | `(imp_block| {$s}) => getStatementM s
+  | _ => throwUnsupportedSyntax
+
+elab "bool%" b:bool_exp ";" : term => do
+  let bVal ← getBoolM b |>.run' {}
+  return toExpr bVal
+
+#eval bool% (!T) && F;
+
+#eval (!true) && false
+
+#eval 3 + 4
+
+#eval bool% 3 ≤ 2 ;
+
+elab "imp%" s:imp_statement : term  => do
+  let stat ← getStatementM s |>.run' {}
+  return toExpr stat
+
+#eval imp% n := 3; m := 4;
+  if (2 ≤ 3) {} else {n := 2;}
